LockProtocol: define generic server send transition

Examples/LockResource/LockProtocol.v
@@ -21,6 +21,15 @@ Variable clients : seq nid.
 Hypothesis Hnin : server \notin clients.
 Hypothesis Huniq : uniq clients.
 
+Lemma client_not_server n : n \in clients -> (n == server) = false.
+Proof.
+  move=>H.
+  case E: (n == server)=>//.
+  move/eqP in E. subst n.
+  move: (Hnin).
+  by rewrite H.
+Qed.
+
 Definition nodes := [:: server] ++ clients.
 
 Notation epoch := nat (only parsing).
@@ -57,19 +66,17 @@ Definition coh_msg pkt e :=
 Definition st := ptr_nat 1.
 
 Definition client_local_coh (cs : client_state) :=
-  [Pred h | valid h /\ h = st :-> cs].
+  [Pred h | h = st :-> cs].
 
 Definition server_local_coh (ss : server_state) :=
-  [Pred h | valid h /\ h = st :-> ss].
+  [Pred h | h = st :-> ss].
 
 Definition local_coh (n : nid) :=
-  [Pred h |
+  [Pred h | valid h /\
    if n == server
    then exists ss, server_local_coh ss h
-   else if n \in clients
-   then exists cs, client_local_coh cs h
-   else True].
-
+   else n \in clients /\
+        exists cs, client_local_coh cs h].
 
 Definition soup_coh : Pred soup :=
   [Pred s |
@@ -125,8 +132,155 @@ Definition client_recv_step (cs : client_state) (from : nid)
   then Held e
   else NotHeld.
 
+Section GetterLemmas.
+
+Lemma getLocal_coh n d (C : LockCoh d):
+  n \in nodes ->
+  valid (getLocal n d) /\
+  if n == server
+  then exists (ss : server_state),
+      getLocal n d = st :-> ss
+  else (n \in clients) /\
+       exists (cs : client_state),
+           getLocal n d = st :-> cs.
+Proof.
+  by case: C=>_ _ _ /(_ n)G; rewrite /local_coh/=.
+Qed.
+
+Lemma getLocal_server_st_tp d (C : LockCoh d) s:
+  find st (getLocal server d) = Some s ->
+  idyn_tp s = server_state.
+Proof.
+have pf: server \in nodes by rewrite inE eqxx.
+move: (getLocal_coh C pf); rewrite eqxx; move =>[V][s']Z; rewrite Z in V *.
+by rewrite hfindPt -(hvalidPt _ s') V; case=><-.
+Qed.
+
+Lemma getLocal_client_st_tp n d (C : LockCoh d) (H : n \in clients) s:
+  find st (getLocal n d) = Some s ->
+  idyn_tp s = client_state.
+Proof.
+have pf: n \in nodes by rewrite inE/= orbC H.
+move: (getLocal_coh C pf); rewrite H=>[[V]].
+rewrite client_not_server//.
+move=>[_][cs] L. rewrite L in V *.
+rewrite hfindPt -(hvalidPt _ cs) V.
+by case=> <-.
+Qed.
+
+Definition getSt_server d (C : LockCoh d) : server_state :=
+  match find st (getLocal server d) as f return _ = f -> _ with
+    Some v => fun epf => icoerce id (idyn_val v) (getLocal_server_st_tp C epf)
+  | _ => fun epf => ServerState [::] 0 None
+  end (erefl _).
+
+Lemma getSt_server_K d (C : LockCoh d) m :
+  getLocal server d = st :-> m -> getSt_server C = m.
+Proof.
+move=>E; rewrite /getSt_server/=.
+have pf: server \in nodes by rewrite inE eqxx.
+have V: valid (getLocal server d) by case: (getLocal_coh C pf).
+move: (getLocal_server_st_tp C); rewrite !E=>/= H.
+by apply: ieqc.
+Qed.
+
+End GetterLemmas.
+
+Section ServerGenericSendTransitions.
+
+Definition HCn this to := (this == server /\ to \in clients).
+
+Variable the_tag : nat.
+
+Variable prec : server_state -> nid -> seq nid -> Prop.
+
+Hypothesis prec_safe :
+  forall this to s m,
+    HCn this to ->
+    prec s to m ->
+    coh_msg (Msg (TMsg the_tag m) this to true) (current_epoch s).
+
+Notation coh := LockCoh.
+
+Definition server_send_safe (this n : nid)
+           (d : dstatelet) (msg : seq nat) :=
+  HCn this n /\
+  exists (C : coh d), prec (getSt_server C) n msg.
+
+Lemma server_send_safe_coh this to d m : server_send_safe this to d m -> coh d.
+Proof. by case=>_[]. Qed.
+
+Lemma server_send_this_in this to : HCn this to -> this \in nodes.
+Proof. by case=>/eqP->; rewrite inE eqxx. Qed.
+
+Lemma server_send_to_in this to : HCn this to -> to \in nodes.
+Proof. by case=>_; rewrite /nodes inE/= orbC=>->. Qed.
+
+Lemma server_send_safe_in this to d m : server_send_safe this to d m ->
+                                  this \in nodes /\ to \in nodes.
+Proof.
+by case=>[]=>G _; move/server_send_to_in: (G)->; case: G=>/eqP-> _; rewrite inE eqxx.
+Qed.
+
+
+Definition server_step (this to : nid) (d : dstatelet)
+           (msg : seq nat)
+           (pf : server_send_safe this to d msg) :=
+  let C := server_send_safe_coh pf in
+  let s := getSt_server C in
+  Some (st :-> server_send_step s to).
+
+Lemma soup_coh_post_msg d m:
+    soup_coh (dsoup d) -> (exists e, coh_msg m e) -> soup_coh (post_msg (dsoup d) m).1.
+Proof.
+move=>[H1 H2][y]Cm; split=>[|i ms/=]; first by rewrite valid_fresh.
+rewrite findUnL; last by rewrite valid_fresh.
+case: ifP=>E; first by move/H2.
+by move/um_findPt_inv=>[Z G]; subst i m; exists y.
+Qed.
+
+Lemma coh_dom_upd this d s :
+  this \in nodes -> coh d -> dom (upd this s (dstate d)) =i nodes.
+Proof.
+move=>D C z; rewrite -(cohDom C) domU inE/=.
+by case: ifP=>///eqP->{z}; rewrite (cohDom C) D; apply: cohVl C.
+Qed.
+
+Lemma server_step_coh : s_step_coh_t coh the_tag server_step.
+Proof.
+move=>this to d msg pf h[]->{h}.
+have C : (coh d) by case: pf=>?[].
+have E: this = server by case: pf=>[][]/eqP.
+split=>/=.
+- apply: soup_coh_post_msg; first by case:(server_send_safe_coh pf).
+  case: (pf)=>H[C']P/=.
+  eexists.
+  by apply: (prec_safe _ P).
+- by apply: coh_dom_upd=>//; case: (server_send_safe_in pf).
+- by rewrite validU; apply: cohVl C.
+move=>n Ni. rewrite /local_coh/=.
+rewrite /getLocal/=findU; case: ifP=>B; last by case: C=>_ _ _/(_ n Ni).
+move/eqP: B=>Z; subst n this; rewrite eqxx (cohVl C)/=.
+split.
+by rewrite hvalidPt.
+by eexists.
+Qed.
+
+Lemma server_step_def this to d msg :
+      server_send_safe this to d msg <->
+      exists b pf, @server_step this to d msg pf = Some b.
+Proof.
+split=>[pf/=|]; last by case=>?[].
+set b := let C := server_send_safe_coh pf in
+         let s := getSt_server C in
+         st :-> (server_send_step s to).
+by exists b, pf.
+Qed.
+
+Definition server_send_trans :=
+  SendTrans server_send_safe_coh server_send_safe_in server_step_def server_step_coh.
+
+End ServerGenericSendTransitions.
 
 End LockProtocol.
 End LockProtocol.
-
-
